Ghost arg and ret in call

Test/VProg.v
@@ -11,27 +11,35 @@ Import VProg._Abbrev.
 Definition f_0 : fid := 0.
 Definition f_1 : fid := 0.
 Definition f_2 : fid := 2.
+Definition f_3 : fid := 3.
+Definition f_4 : fid := 4.
 
 Definition sig_0 := mk_f_sig (ptr * ptr) unit.
 Definition sig_1 := mk_f_sig (ptr * ptr * ptr) unit.
 Definition sig_2 := mk_f_sig (ptr * ptr * ptr) ptr.
+Definition sig_3 := mk_f_sig ptr ptr.
+Definition sig_4 := mk_f_sig (ptr * ptr) ptr.
 
 Definition SIG : sig_context :=
   fun f => match f with
   | 0 => Some sig_0
   | 1 => Some sig_1
   | 2 => Some sig_2
+  | 3 => Some sig_3
+  | 4 => Some sig_4
   | _ => None
   end.
 
-Definition spec_0 : FSpec sig_0 (fun '(p0, p1) =>
+Definition sigh_0 := mk_f_sigh sig_0 None None.
+Definition spec_0 : FSpec sigh_0 (fun '(p0, p1) =>
   Spec.Expanded.mk_r0 (fun '(n0, n1) =>
   Spec.Expanded.mk_r1 [] [CTX.mka (SLprop.cell p0, n0); CTX.mka (SLprop.cell p1, n1)] True (fun _ =>
   Spec.Expanded.mk_r2 (fun 'tt =>
   Spec.Expanded.mk_r3 [CTX.mka (SLprop.cell p0, n1); CTX.mka (SLprop.cell p1, n0)] True)))).
 Proof. Tac.build_FSpec. Defined.
 
-Definition spec_1 : FSpec sig_1 (fun '(p0, p1, p2) =>
+Definition sigh_1 := mk_f_sigh sig_1 None None.
+Definition spec_1 : FSpec sigh_1 (fun '(p0, p1, p2) =>
   Spec.Expanded.mk_r0 (fun '(n0, n1, n2) =>
   Spec.Expanded.mk_r1 [CTX.mka (SLprop.cell p2, n2)]
     [CTX.mka (SLprop.cell p0, n0); CTX.mka (SLprop.cell p1, n1)] True (fun _ =>
@@ -39,55 +47,79 @@ Definition spec_1 : FSpec sig_1 (fun '(p0, p1, p2) =>
   Spec.Expanded.mk_r3 [CTX.mka (SLprop.cell p0, n1); CTX.mka (SLprop.cell p1, n0)] True)))).
 Proof. Tac.build_FSpec. Defined.
 
-Definition spec_2 : FSpec sig_2 (fun '(p0, p1, p2) =>
+Definition sigh_2 := mk_f_sigh sig_2 None None.
+Definition spec_2 : FSpec sigh_2 (fun '(p0, p1, p2) =>
   Spec.Expanded.mk_r0 (fun '(n0, n1, n2) =>
-  Spec.Expanded.mk_r1 [CTX.mka (SLprop.cell p2, n2)]
+  Spec.Expanded.mk_r1 (GO := None) [CTX.mka (SLprop.cell p2, n2)]
              [CTX.mka (SLprop.cell p0, n0); CTX.mka (SLprop.cell p1, n1)] True (fun p =>
   Spec.Expanded.mk_r2 (fun '(n, n1') =>
   Spec.Expanded.mk_r3 [CTX.mka (SLprop.cell p, n); CTX.mka (SLprop.cell p1, n1')] (n1' > 0))))).
-Proof.
-  Tac.build_FSpec.
-Defined.
+Proof. Tac.build_FSpec. Defined.
+
+Definition sigh_3 := mk_f_sigh sig_3 (Some (fun _ => ptr)) (Some (fun _ => ptr)).
+Definition spec_3 : FSpec sigh_3 (fun p0 p1 =>
+  Spec.Expanded.mk_r0 (fun '(n0, n1) =>
+  Spec.Expanded.mk_r1 (GO := Some _) []
+             [CTX.mka (SLprop.cell p0, n0); CTX.mka (SLprop.cell p1, n1)] True (fun r =>
+  Spec.Expanded.mk_r2 (fun '(n0', n1') =>
+  Spec.Expanded.mk_r3
+             [CTX.mka (SLprop.cell (CP.projG1 r), n0'); CTX.mka (SLprop.cell (CP.projG2 r), n1')] True)))).
+Proof. Tac.build_FSpec. Defined.
+
+Definition sigh_4 := mk_f_sigh sig_4 None (Some (fun _ => ptr)).
+Definition spec_4 : FSpec sigh_4 (fun '(p0, p1) =>
+  Spec.Expanded.mk_r0 (fun '(n0, n1) =>
+  Spec.Expanded.mk_r1 (GO := Some _) []
+             [CTX.mka (SLprop.cell p0, n0); CTX.mka (SLprop.cell p1, n1)] True (fun r =>
+  Spec.Expanded.mk_r2 (fun '(n0', n1') =>
+  Spec.Expanded.mk_r3
+             [CTX.mka (SLprop.cell (CP.projG1 r), n0'); CTX.mka (SLprop.cell (CP.projG2 r), n1')] True)))).
+Proof. Tac.build_FSpec. Defined.
 
 Definition SPEC : CP.spec_context SIG :=
   fun f => match f with
   | 0 => cp_f_spec (m_spec spec_0)
   | 1 => cp_f_spec (m_spec spec_1)
   | 2 => cp_f_spec (m_spec spec_2)
+  | 3 => cp_f_spec (m_spec spec_3)
+  | 4 => cp_f_spec (m_spec spec_4)
   | _ => tt
   end.
 
 Definition HSPC_f_0 := cp_has_spec SPEC f_0 eq_refl eq_refl.
+Definition HSPC_f_3 := cp_has_spec SPEC f_3 eq_refl eq_refl.
 
 
-Definition vprog_0 : f_body SPEC sig_0 := fun '(p0, p1) =>
+Definition vprog_0 : f_body SPEC sigh_0 := fun '(p0, p1) =>
   Bind _ (Read  _ p0)    (fun v0 =>
   Bind _ (Read  _ p1)    (fun v1 =>
   Bind _ (Write _ p0 v1) (fun _  =>
          (Write _ p1 v0) ))).
 
-Definition vprog_1 : f_body SPEC sig_1 := fun '(p0, p1, p2) =>
-  Call (sg := sig_0) _ f_0 eq_refl (p0, p1) _ (HSPC_f_0 _).
+Definition vprog_1 : f_body SPEC sigh_1 := fun '(p0, p1, p2) =>
+  Call _ f_0 eq_refl sigh_0 (p0, p1) tt _ (HSPC_f_0 _).
 
 Definition data42 : nat := 42.
 
-Definition vprog_2 : f_body SPEC sig_2 := fun '(p0, p1, p2) =>
+Definition vprog_2 : f_body SPEC sigh_2 := fun '(p0, p1, p2) =>
   Bind _ (Read  _ p0) (fun v0 =>
   Bind _ (Write _ p1 data42) (fun _ =>
   Bind _ (Assert _ (fun '(v0', v1') =>
     ([CTX.mka (SLprop.cell p0, v0'); CTX.mka (SLprop.cell p1, v1')], v0' = v0))) (fun _ =>
   Ret _ p0 (fun p => [Vprop.mk (SLprop.cell p)])))).
 
-Definition impl_2 (ps : ptr * ptr * ptr) :
-  { i : CP.instr ptr | i = i_impl (vprog_2 ps) }.
-Proof.
-  unfold i_impl, vprog_2; cbn.
-  case ps as ((p0, p1), p2); cbn.
-  eexists. reflexivity.
-Defined.
+Definition vprog_3 : f_body SPEC sigh_3 := fun p0 p1 =>
+  Ret _ (CP.existG _ p0 p1)
+        (fun r => [Vprop.mk (SLprop.cell (CP.projG1 r)); Vprop.mk (SLprop.cell (CP.projG2 r))]).
+
+Definition vprog_4 : f_body SPEC sigh_4 := fun '(p0, p1) =>
+  Bind _ (Call _ f_3 eq_refl sigh_3 p0 p1 _ (HSPC_f_3 _)) (fun '(CP.existG _ p0' p1') =>
+  Ret _ (CP.existG _ p0' p1')
+        (fun r => [Vprop.mk (SLprop.cell (CP.projG1 r)); Vprop.mk (SLprop.cell (CP.projG2 r))])).
+
 
 Lemma imatch_0:
-  f_body_match SPEC vprog_0 (m_spec spec_0).
+  f_body_match vprog_0 (m_spec spec_0).
 Proof.
   intros (p0, p1).
   Tac.build_impl_match.
@@ -96,12 +128,12 @@ Proof.
   tauto.
 Qed.
 
-Definition cp_0: f_impl _ vprog_0.
+Definition cp_0: f_impl vprog_0.
 Proof. Tac.extract_impl. Defined.
 
 
 Lemma imatch_1:
-  f_body_match SPEC vprog_1 (m_spec spec_1).
+  f_body_match vprog_1 (m_spec spec_1).
 Proof.
   intros ((p0, p1), p2).
   Tac.build_impl_match.
@@ -110,11 +142,11 @@ Proof.
   tauto.
 Qed.
 
-Definition cp_1: f_impl _ vprog_1.
+Definition cp_1: f_impl vprog_1.
 Proof. Tac.extract_impl. Defined.
 
 Lemma imatch_2:
-  f_body_match SPEC vprog_2 (m_spec spec_2).
+  f_body_match vprog_2 (m_spec spec_2).
 Proof.
   intros ((p0, p1), p2).
   Tac.build_impl_match.
@@ -124,23 +156,87 @@ Proof.
   unfold data42; repeat constructor.
 Qed.
 
-Definition cp_2: f_impl _ vprog_2.
+Definition cp_2: f_impl vprog_2.
 Proof. Tac.extract_impl. Defined.
 
 
-Definition sig_a0 := mk_f_sig (ptr * ptr) unit.
-Definition spec_a0 : FSpec sig_a0 (fun ps =>
+Lemma imatch_3:
+  f_body_match vprog_3 (m_spec spec_3).
+Proof.
+  intros p0.
+  Tac.build_impl_match.
+  FP.simpl_prog.
+  FP.by_wlp.
+  tauto.
+Qed.
+
+Definition cp_3: f_impl vprog_3.
+Proof. Tac.extract_impl. Defined.
+
+Lemma imatch_4:
+  f_body_match vprog_4 (m_spec spec_4).
+Proof.
+  intros (p0, p1).
+  Tac.build_impl_match.
+  FP.simpl_prog.
+  FP.by_wlp.
+  tauto.
+Qed.
+
+Definition cp_4: f_impl vprog_4.
+Proof. Tac.extract_impl. Defined.
+
+
+Definition IMPL : CP.impl_context SIG :=
+  fun f => match f with
+  | 0 => proj1_sig cp_0
+  | 1 => proj1_sig cp_1
+  | 2 => proj1_sig cp_2
+  | 3 => proj1_sig cp_3
+  | 4 => proj1_sig cp_4
+  | _ => tt
+  end.
+
+Ltac case_until_True :=
+  try exact (fun _ => Logic.I);
+  let i := fresh "i" in
+  intros [|i]; [|revert i; case_until_True].
+
+Lemma match_context:
+  CP.context_match_spec IMPL SPEC.
+Proof.
+  case_until_True;
+  cbn beta iota delta [SIG IMPL SPEC];
+  apply f_impl_match_spec.
+  - apply imatch_0.
+  - apply imatch_1.
+  - apply imatch_2.
+  - apply imatch_3.
+  - apply imatch_4.
+Qed.
+
+Lemma context_oracle_free:
+  CP.context_oracle_free IMPL.
+Proof.
+  case_until_True;
+  cbn beta iota delta [SIG IMPL SPEC];
+  apply f_impl_oracle_free.
+Qed.
+
+
+Definition sigh_a0 := mk_f_sig1 (ptr * ptr) None unit None.
+Definition spec_a0 : FSpec sigh_a0 (fun ps =>
   Spec.Expanded.mk_r0 (fun n =>
   Spec.Expanded.mk_r1 [CTX.mka (SLprop.cell (fst ps), n)] [] True (fun _ =>
   Spec.Expanded.mk_r2 (fun 'tt =>
   Spec.Expanded.mk_r3 [] True)))).
 Proof. Tac.build_FSpec. Defined.
 
-Definition vprog_a0 : f_body SPEC sig_a0 := fun ps =>
+Definition vprog_a0 : f_body SPEC sigh_a0 := fun ps =>
   Bind _ (let (p0, _) := ps in Read _ p0) (fun v0 =>
   Ret _ tt (fun _ => [])).
 Lemma imatch_a0:
-  f_body_match SPEC vprog_a0 (m_spec spec_a0).
+  f_body_match vprog_a0 (m_spec spec_a0).
 Proof.
   intro ps.
   Tac.build_impl_match.
@@ -149,12 +245,12 @@ Proof.
   cbn. tauto.
 Qed.
 
-Definition cp_a0: f_impl _ vprog_a0.
+Definition cp_a0: f_impl vprog_a0.
 Proof. Tac.extract_impl. Defined.
 
 
-Definition sig_a1a := mk_f_sig (bool * ptr * ptr * ptr) unit.
-Definition spec_a1a : FSpec sig_a1a (fun '(b, p0, p1, p2) =>
+Definition sigh_a1a := mk_f_sig1 (bool * ptr * ptr * ptr) None unit None.
+Definition spec_a1a : FSpec sigh_a1a (fun '(b, p0, p1, p2) =>
   Spec.Expanded.mk_r0 (fun '(n0, n1, n2) =>
   Spec.Expanded.mk_r1 [CTX.mka (SLprop.cell p0, n0)] [CTX.mka (SLprop.cell p1, n1); CTX.mka (SLprop.cell p2, n2)]
     True (fun _ =>
@@ -163,87 +259,41 @@ Definition spec_a1a : FSpec sig_a1a (fun '(b, p0, p1, p2) =>
     (b = true -> n1' = 0))))).
 Proof. Tac.build_FSpec. Defined.
 
-Definition vprog_a1a : f_body SPEC sig_a1a := fun '(b, p0, p1, p2) =>
+Definition vprog_a1a : f_body SPEC sigh_a1a := fun '(b, p0, p1, p2) =>
   if b
   then Write _ p1 0
   else Write _ p2 1.
 Lemma imatch_a1a:
-  f_body_match SPEC vprog_a1a (m_spec spec_a1a).
+  f_body_match vprog_a1a (m_spec spec_a1a).
 Proof.
   intros (((b, p0), p1), p2).
   Tac.build_impl_match.
-  (*
-  Tac.build_impl_match_init.
-  refine (transform_spec _ _ _).
-  - Tac.build_HasSpec_branch ltac:(fun _ => Tac.build_HasSpec) b.
-    (*
-    refine (transform_spec _ _ _).
-    + (* For each branch a specification where [sf_csm] and [sf_prd] do not depend on the
-         arguments of the matched value. *)
-      lazymatch goal with |- HasSpec _ _ _ ?s =>
-        Tac.build_term s ltac:(fun _ =>
-          simple refine (mk_i_spec _ _ _);
-          [ (* sf_csm  *) cbn; Tac.const_case b; clear
-          | (* sf_prd  *) cbn; Tac.const_case b; clear b
-          | (* sf_spec *) case b; clear b ];
-          shelve)
-      end;
-      cbn.
-      case b;
-      (simple refine (VProg.Tac.change_arg _ _ _ _);
-       [ shelve | Tac.build_HasSpec | Tac.build_i_spec_t_eq ]).
-    + cbn.
-      simple refine (intro_TrSpec_branch _ _ _ _ _).
-      1,2:clear; shelve.
-      1:shelve.
-      { (* f1 *) Tac.nondep_case b; clear b; shelve. }
-      { (* C  *)
-        case b;
-        match goal with |- branch_collect_csm ?c ?cs =>
-          Tac.elist_add cs c; constructor
-        end.
-      }
-      { (* E *)
-        match goal with |- _ = List.fold_left _ ?cs _ =>
-          Tac.elist_end cs
-        end.
-        cbn. reflexivity.
-      }
-      cbn.
-      case b.
-      * refine (TrSpec_branch_0 _ _); Tac.build_i_spec_t_eq.
-      * Tac.build_Tr_change_exact.
-    *)
-  - Tac.build_Tr_change_exact.
-  *)
-  - (* WLP     *)
-    cbn.
-    FP.simpl_prog.
-    FP.by_wlp.
-    intuition congruence.
+  FP.simpl_prog.
+  FP.by_wlp.
+  intuition congruence.
 Qed.
 
-Definition cp_a1a: f_impl _ vprog_a1a.
+Definition cp_a1a: f_impl vprog_a1a.
 Proof. Tac.extract_impl. Defined.
 
 
 Inductive bool3 : Set := B0 | B1 | B2.
 
-Definition sig_a1b := mk_f_sig (bool3 * ptr) unit.
-Definition spec_a1b : FSpec sig_a1b (fun '(b, p) =>
+Definition sigh_a1b := mk_f_sig1 (bool3 * ptr) None unit None.
+Definition spec_a1b : FSpec sigh_a1b (fun '(b, p) =>
   Spec.Expanded.mk_r0 (fun n =>
   Spec.Expanded.mk_r1 [] [CTX.mka (SLprop.cell p, n)] (b <> B2) (fun _ =>
   Spec.Expanded.mk_r2 (fun n' =>
   Spec.Expanded.mk_r3 [CTX.mka (SLprop.cell p, n')] (b <> B1 -> n' = 0))))).
 Proof. Tac.build_FSpec. Defined.
 
-Definition vprog_a1b : f_body SPEC sig_a1b := fun '(b, p) =>
+Definition vprog_a1b : f_body SPEC sigh_a1b := fun '(b, p) =>
   match b with
   | B0 => Write _ p 0
   | B1 | B2 => Ret _ tt (fun _ => [])
   end.
 Lemma imatch_a1b:
-  f_body_match SPEC vprog_a1b (m_spec spec_a1b).
+  f_body_match vprog_a1b (m_spec spec_a1b).
 Proof.
   intros (b, p).
   Tac.build_impl_match.
@@ -253,8 +303,8 @@ Proof.
 Qed.
 
 
-Definition sig_a1c := mk_f_sig (option nat * ptr) unit.
-Definition spec_a1c : FSpec sig_a1c (fun '(o, p) =>
+Definition sigh_a1c := mk_f_sig1 (option nat * ptr) None unit None.
+Definition spec_a1c : FSpec sigh_a1c (fun '(o, p) =>
   Spec.Expanded.mk_r0 (fun n =>
   Spec.Expanded.mk_r1 [] [CTX.mka (SLprop.cell p, n)]
     (n > 0 /\ match o with Some n' => n' > 0 | None => True end) (fun _ =>
@@ -262,13 +312,13 @@ Definition spec_a1c : FSpec sig_a1c (fun '(o, p) =>
   Spec.Expanded.mk_r3 [CTX.mka (SLprop.cell p, n')] (n' > 0))))).
 Proof. Tac.build_FSpec. Defined.
 
-Definition vprog_a1c : f_body SPEC sig_a1c := fun '(o, p) =>
+Definition vprog_a1c : f_body SPEC sigh_a1c := fun '(o, p) =>
   match o with
   | Some n => Write _ p n
   | None   => Ret _ tt (fun _ => [])
   end.
 Lemma imatch_a1c:
-  f_body_match SPEC vprog_a1c (m_spec spec_a1c).
+  f_body_match vprog_a1c (m_spec spec_a1c).
 Proof.
   intros (o, p).
   Tac.build_impl_match.
@@ -278,8 +328,8 @@ Proof.
 Qed.
 
 
-Definition sig_a2a := mk_f_sig (ptr * ptr) unit.
-Definition spec_a2a : FSpec sig_a2a (fun '(p0, p1) =>
+Definition sigh_a2a := mk_f_sig1 (ptr * ptr) None unit None.
+Definition spec_a2a : FSpec sigh_a2a (fun '(p0, p1) =>
   Spec.Expanded.mk_r0 (fun '(n0, n1) =>
   Spec.Expanded.mk_r1 [CTX.mka (SLprop.cell p0, n0)] [CTX.mka (SLprop.cell p1, n1)]
     (n0 <= n1) (fun _ =>
@@ -287,13 +337,13 @@ Definition spec_a2a : FSpec sig_a2a (fun '(p0, p1) =>
   Spec.Expanded.mk_r3 [CTX.mka (SLprop.cell p1, n1')] (n0 <= n1'))))).
 Proof. Tac.build_FSpec. Defined.
 
-Definition vprog_a2a : f_body SPEC sig_a2a := fun '(p0, p1) =>
+Definition vprog_a2a : f_body SPEC sigh_a2a := fun '(p0, p1) =>
   Bind _ (Read _ p1) (fun v1 =>
   Bind _ (GGet _ (SLprop.cell p0)) (fun v0 =>
   Bind _ (Assert _ (fun 'tt => ([], v0 <= v1))) (fun _ =>
           Write _ p1 (S v1)))).
 Lemma imatch_a2a:
-  f_body_match SPEC vprog_a2a (m_spec spec_a2a).
+  f_body_match vprog_a2a (m_spec spec_a2a).
 Proof.
   intros (p0, p1).
   Tac.build_impl_match.
@@ -301,17 +351,17 @@ Proof.
   FP.by_wlp.
   intuition.
 Qed.
-Definition cp_a2a: f_impl _ vprog_a2a.
+Definition cp_a2a: f_impl vprog_a2a.
 Proof. Tac.extract_impl. Defined.
 
-Definition vprog_a2b : f_body SPEC sig_a2a := fun '(p0, p1) =>
+Definition vprog_a2b : f_body SPEC sigh_a2a := fun '(p0, p1) =>
   Bind _ (Bind _ (Read _ p1) (fun v1 =>
           Bind _ (GGet _ (SLprop.cell p0)) (fun v0 =>
           Ret _ (CP.existG _ v1 v0) (fun _ => [])))) (fun '(CP.existG _ v1 v0) =>
   Bind _ (Assert _ (fun 'tt => ([], v0 <= v1))) (fun _ =>
           Write _ p1 (S v1))).
 Lemma imatch_a2b:
-  f_body_match SPEC vprog_a2b (m_spec spec_a2a).
+  f_body_match vprog_a2b (m_spec spec_a2a).
 Proof.
   intros (p0, p1).
   Tac.build_impl_match.
@@ -319,5 +369,28 @@ Proof.
   FP.by_wlp.
   intuition.
 Qed.
-Definition cp_a2b: f_impl _ vprog_a2b.
+Definition cp_a2b: f_impl vprog_a2b.
+Proof. Tac.extract_impl. Defined.
+
+
+Definition sigh_a3 := mk_f_sig1 unit (Some (fun _ => (nat * nat)%type <: Type)) unit (Some (fun _ => nat <: Type)).
+Definition spec_a3 : FSpec sigh_a3 (fun _ '(n0, n1) =>
+  Spec.Expanded.mk_r0 (fun 'tt =>
+  Spec.Expanded.mk_r1 (GO := Some _) [] [] True (fun r =>
+  Spec.Expanded.mk_r2 (fun 'tt =>
+  Spec.Expanded.mk_r3 [] (CP.projG2 r = n0 + n1))))).
+Proof. Tac.build_FSpec. Defined.
+
+Definition vprog_a3 : f_body SPEC sigh_a3 := fun _ '(n0, n1) =>
+  Ret _ (CP.existG _ tt (n0 + n1)) (fun _ => []).
+Lemma imatch_a3:
+  f_body_match vprog_a3 (m_spec spec_a3).
+Proof.
+  intros _arg.
+  Tac.build_impl_match.
+  FP.simpl_prog.
+  FP.by_wlp.
+  tauto.
+Qed.
+Definition cp_a3: f_impl vprog_a3.
 Proof. Tac.extract_impl. Defined.
